

3) a) For a matrix to be orthogonal, it should satisfy the following:

$$\underline{Q}^{-1} = \underline{Q}^T, \text{ i.e. inverse of } \underline{Q} = \text{transpose of } \underline{Q}$$

First let us calculate \underline{Q}^T :- \underline{Q} is given as $(\underline{I} - \underline{S})^{-1}(\underline{I} + \underline{S})$

$$\begin{aligned}\underline{Q}^T &= [(\underline{I} + \underline{S})^{-1}(\underline{I} + \underline{S})]^T \\&= (\underline{I} + \underline{S})^T [(\underline{I} - \underline{S})^{-1}]^T \quad (\text{reversal law, i.e. } (\underline{AB})^T = \underline{B}^T \underline{A}^T) \\&= (\underline{I}^T + \underline{S}^T) [(\underline{I} - \underline{S})^{-1}]^T \quad (\underline{A+B}^T = \underline{A}^T + \underline{B}^T) \\&= (\underline{I}^T + \underline{S}^T) [(\underline{I} - \underline{S})^T]^{-1} \quad ((\underline{A}^{-1})^T = (\underline{A}^T)^{-1}) \\&= (\underline{I} - \underline{S}) (\underline{I}^T - \underline{S}^T)^{-1} \quad (\underline{I}^T = \underline{I} \text{ and } \underline{S}^T = -\underline{S}) \\&= (\underline{I} - \underline{S}) (\underline{I} + \underline{S})^{-1}\end{aligned}$$

To prove \underline{Q} 's orthogonality, we should prove $\underline{Q} \cdot \underline{Q}^T = \underline{I}$. For this we need to rearrange ~~\underline{Q} & \underline{Q}^T~~

Proof of commutability:

In this proof, I want to prove that $(\underline{I} + \underline{S})(\underline{I} - \underline{S}) = (\underline{I} - \underline{S})(\underline{I} + \underline{S})$

$$\begin{aligned}(\underline{I} + \underline{S})(\underline{I} - \underline{S}) &= \underline{I}^2 + \underline{S} - \underline{S} - \underline{S}^2 = \underline{I} - \underline{S}^2 \\(\underline{I} - \underline{S})(\underline{I} + \underline{S}) &= \underline{I}^2 - \underline{S} + \underline{S} - \underline{S}^2 = \underline{I} - \underline{S}^2\end{aligned}$$

∴ Hence, the commutability is proved.

This proof shall help us to rearrange \underline{Q} & \underline{Q}^T .

Rearranging Q^T :

For this, we have to ~~prove~~ ^{use the} proven commutability:

$$(\underline{I} - \underline{S})(\underline{I} + \underline{S}) = (\underline{I} + \underline{S})(\underline{I} - \underline{S})$$

$$(\underline{I} - \underline{S})^{-1}(\underline{I} - \underline{S})(\underline{I} + \underline{S}) = (\underline{I} - \underline{S})^{-1}(\underline{I} + \underline{S})(\underline{I} - \underline{S}) \quad (\text{Left multiply by } (\underline{I} - \underline{S})^{-1})$$

$$\underline{I}(\underline{I} + \underline{S}) = (\underline{I} - \underline{S})^{-1}(\underline{I} + \underline{S})(\underline{I} - \underline{S})$$

$$(\underline{I} + \underline{S})(\underline{I} - \underline{S})^{-1} = (\underline{I} - \underline{S})^{-1}(\underline{I} + \underline{S})(\underline{I} - \underline{S})(\underline{I} - \underline{S})^{-1} \quad (\text{Right multiply by } (\underline{I} - \underline{S})^{-1})$$

$$(\underline{I} + \underline{S})(\underline{I} - \underline{S})^{-1} = (\underline{I} - \underline{S})^{-1}(\underline{I} + \underline{S})$$

Hence, \underline{Q} can be written as ~~$(\underline{I} - \underline{S})^{-1}(\underline{I} + \underline{S})$~~
 $(\underline{I} + \underline{S})(\underline{I} - \underline{S})^{-1}$.

Now, we can prove $\underline{Q}^T \cdot \underline{Q} = \underline{I}$

$$\underline{Q}^T \underline{Q} = [(\underline{I} - \underline{S})(\underline{I} + \underline{S})^{-1}] [(\underline{I} + \underline{S})(\underline{I} - \underline{S})^{-1}]$$

$$= (\underline{I} - \underline{S}) \left[(\underline{I} + \underline{S})^{-1} (\underline{I} + \underline{S}) \right] (\underline{I} - \underline{S})^{-1} \quad (\text{distributive property of matrix multiplication})$$

$$= (\underline{I} - \underline{S})(\underline{I})(\underline{I} - \underline{S})^{-1}$$

$$= (\underline{I} - \underline{S})(\underline{I} - \underline{S})^{-1}$$

$$= \underline{I}$$

\therefore Hence proven, $\underline{Q}^T = \underline{Q}$, or long as \underline{S} is skew-symmetric

3.b) Since this is an "if & only if" statement, we shall have to prove both ways.

Proof #1: If $\underline{\underline{S}} = \underline{\underline{0}}$, then $\underline{\underline{u}}^T \underline{\underline{S}} \underline{\underline{u}} = \underline{\underline{0}}$.

This is easy to prove. If $\underline{\underline{S}} = \underline{\underline{0}}$, then

$$\begin{aligned} \underline{\underline{u}}^T \underline{\underline{S}} \underline{\underline{u}} &= (\underline{\underline{u}}^T \underline{\underline{S}}) \underline{\underline{u}} && \text{(Distributive property of} \\ &= (\underline{\underline{u}}^T \underline{\underline{0}}) \underline{\underline{u}} && \text{matrix vector multiplication)} \\ &= \underline{\underline{0}} \cdot \underline{\underline{u}} \\ &= \underline{\underline{0}} && \text{(proven)} \end{aligned}$$

Proof #2: If $\underline{\underline{u}}^T \underline{\underline{S}} \underline{\underline{u}} = \underline{\underline{0}}$, then $\underline{\underline{S}} = \underline{\underline{0}}$

This proof has to be done in two stages. In the first stage, we need to prove that all diagonal elements of $\underline{\underline{S}}$ are 0. In the second phase, we prove all non-diagonal elements of $\underline{\underline{S}}$ to be 0. This shall hence prove $\underline{\underline{S}} = \underline{\underline{0}}$.

Phase #1: Prove $\{S_{ii} = 0 \mid \forall i=j\}$

Assume $\underline{\underline{u}} = \underline{\underline{e}}_i$, then ($\underline{\underline{e}}_i$ represents a canonical basis vector)

$$\underline{\underline{e}}_i^T \underline{\underline{S}} \underline{\underline{e}}_i = 0$$

$$S_{ii} = 0 \quad (S_{ii} = \underline{\underline{e}}_i^T \underline{\underline{S}} \underline{\underline{e}}_i)$$

Since i can be any index $1 \leq i \leq m$, all diagonal elements of $\underline{\underline{S}}$ are hence proven to be 0.

Hence, $S_{ii} = 0$.

Phase #2: Prove all non-diagonal elements of \underline{S} are 0.

Assume $\underline{u} = \underline{e}_i + \underline{e}_j$ & $i \neq j$

$$\text{Hence } \underline{u}^T \underline{S} \underline{u} = (\underline{e}_i + \underline{e}_j)^T \underline{S} (\underline{e}_i + \underline{e}_j)$$

$$0 = \underline{e}_i^T \underline{S} \underline{e}_i + \underline{e}_j^T \underline{S} \underline{e}_j + \underline{e}_i^T \underline{S} \underline{e}_j + \underline{e}_j^T \underline{S} \underline{e}_i$$

$$(\underline{S}_{ii} \& \underline{S}_{jj} \text{ are } 0, \text{ as proven in phase \#1}) \quad 0 = \underline{S}_{ii} + \underline{S}_{jj} + \underline{S}_{ij} + \underline{S}_{ji}$$

0, as proven

in phase #1)

$$0 = \underline{S}_{ij} + \underline{S}_{ji}$$

$$(\underline{S}_{ij} = \underline{S}_{ji}, \quad 0 = 2\underline{S}_{ij})$$

because \underline{S}

$$\underline{S}_{ij} = 0$$

is given to be

symmetric)

Hence, $\underline{S}_{ij} = 0$ for $i \neq j$.

Combining results of both phases, it can be stated that $\underline{S} = \underline{\underline{0}}$.

c) ~~Strong~~ Because this statement is an "if & only if" statement, both directions need to be proven.

Proof #1: If \underline{S} is skew symmetric, $\underline{u}^T \underline{S} \underline{u} = 0$.

~~Proof~~ We know that $(\underline{u}^T \underline{S} \underline{u}) = (\underline{u}^T \underline{S} \underline{u})^T$ because $\underline{u}^T \underline{S} \underline{u}$ is a 1×1 matrix, i.e. a scalar value, which has no effect on transpose.

(contd.)

$$\underline{\underline{u}}^T \underline{\underline{S}} \underline{\underline{u}} = (\underline{\underline{u}}^T \underline{\underline{S}} \underline{\underline{u}})^T$$

$$\underline{\underline{u}}^T \underline{\underline{S}} \underline{\underline{u}} = \underline{\underline{u}}^T \underline{\underline{S}}^T (\underline{\underline{u}}^T)^T \quad (\text{Law of reversal, i.e. } (ABC)^T = C^T B^T A^T)$$

$$\underline{\underline{u}}^T \underline{\underline{S}} \underline{\underline{u}} = \underline{\underline{u}}^T \underline{\underline{S}}^T \underline{\underline{u}} \quad ((\underline{\underline{u}}^T)^T = \underline{\underline{u}})$$

$$\underline{\underline{u}}^T \underline{\underline{S}} \underline{\underline{u}} = \underline{\underline{u}}^T (-\underline{\underline{S}}) \underline{\underline{u}} \quad (\text{Since } \underline{\underline{S}} \text{ is skew-symmetric, } \underline{\underline{S}}^T = -\underline{\underline{S}})$$

$$\underline{\underline{u}}^T \underline{\underline{S}} \underline{\underline{u}} = -\underline{\underline{u}}^T \underline{\underline{S}} \underline{\underline{u}}$$

$$x = -x \quad (\text{Assume } x = \underline{\underline{u}}^T \underline{\underline{S}} \underline{\underline{u}})$$

$$2x = 0$$

$$x = 0$$

(Hence proven)

\therefore If $\underline{\underline{S}}$ is skew-symmetric, then $x = \underline{\underline{u}}^T \underline{\underline{S}} \underline{\underline{u}} = 0$.

Proof #2: If $\underline{\underline{u}}^T \underline{\underline{S}} \underline{\underline{u}} = 0$, then $\underline{\underline{S}}$ is skew-symmetric.

Any square matrix can be split into a symmetric & skew symmetric portion as follows:

$$\underline{\underline{A}} = \underbrace{\frac{1}{2}(\underline{\underline{A}} + \underline{\underline{A}}^T)}_{\text{symmetric part}} + \underbrace{\frac{1}{2}(\underline{\underline{A}} - \underline{\underline{A}}^T)}_{\text{skew-symmetric part}}$$

Hence, $\underline{\underline{S}}$ can be represented as $\frac{1}{2}(\underline{\underline{S}} + \underline{\underline{S}}^T) + \frac{1}{2}(\underline{\underline{S}} - \underline{\underline{S}}^T)$.

If we assume $\underline{\underline{S}}_{\text{symm}} = \frac{1}{2}(\underline{\underline{S}} + \underline{\underline{S}}^T)$ and $\underline{\underline{S}}_{\text{skew}} = \frac{1}{2}(\underline{\underline{S}} - \underline{\underline{S}}^T)$.

$\underline{\underline{S}}$ can be re-written as $\underline{\underline{S}}_{\text{symm}} + \underline{\underline{S}}_{\text{skew}}$.

Hence, $\underline{u}^T \underline{S} \underline{u} = 0$

$$\underline{u}^T (\underline{S}_{\text{symm}} + \underline{S}_{\text{skew}}) \underline{u} = 0$$

$$\underline{u}^T \underline{S}_{\text{symm}} \underline{u} + \underline{u}^T \underline{S}_{\text{skew}} \underline{u} = 0$$

$$\underline{u}^T \underline{S}_{\text{symm}} \underline{u} = 0$$

(Because $\underline{u}^T \underline{S}_{\text{skew}} \underline{u} = 0$ as proven in proof #1 of Question 3) a))

$$\therefore \underline{S}_{\text{symm}} = \underline{0}$$

(This has been proven in proof #2 of Question 3) b))

$$\frac{1}{2} (\underline{S} + \underline{S}^T) = \underline{0} \quad (\text{Substituting definition of } \underline{S}_{\text{symm}})$$

$$\underline{S} + \underline{S}^T = \underline{0}$$

$$\underline{S}^T = -\underline{S}$$

Since this is the fundamental property of a skew-symmetric matrix, we can henceforth prove that \underline{S} is a skew-symmetric matrix.